pulse/pulse2rust/src/Pulse2Rust.fst
@@ -93,6 +93,9 @@ let rec extract_mlty (g:env) (t:S.mlty) : typ =
     when S.string_of_mlpath p = "Pulse.Lib.Rust.Slice.slice" ->
     let is_mut = true in
     arg |> extract_mlty g |> mk_slice_typ |> mk_ref_typ is_mut
+  | S.MLTY_Named ([arg], p)
+    when S.string_of_mlpath p = "Pulse.Lib.Rust.Vec.vec" ->
+    arg |> extract_mlty g |> mk_vec_typ
   | S.MLTY_Erased -> mk_scalar_typ "unit"
   | _ -> fail_nyi (format1 "mlty %s" (S.mlty_to_string t))
 
@@ -205,14 +208,25 @@ let rec extract_mlexpr (g:env) (e:S.mlexpr) : expr =
     if b then e
     else mk_ref_read e
   | S.MLE_App ({expr=S.MLE_TApp ({expr=S.MLE_Name p}, [_])}, [e; i; _; _])
-    when S.string_of_mlpath p = "Pulse.Lib.Rust.Slice.op_Array_Access" ->
+    when S.string_of_mlpath p = "Pulse.Lib.Rust.Slice.op_Array_Access" ||
+         S.string_of_mlpath p = "Pulse.Lib.Rust.Vec.op_Array_Access" ->
     mk_expr_index (extract_mlexpr g e) (extract_mlexpr g i)
   | S.MLE_App ({expr=S.MLE_TApp ({expr=S.MLE_Name p}, [_])}, [e1; e2; e3; _])
-    when S.string_of_mlpath p = "Pulse.Lib.Rust.Slice.op_Array_Assignment" ->
+    when S.string_of_mlpath p = "Pulse.Lib.Rust.Slice.op_Array_Assignment" ||
+         S.string_of_mlpath p = "Pulse.Lib.Rust.Vec.op_Array_Assignment" ->
     let e1 = extract_mlexpr g e1 in
     let e2 = extract_mlexpr g e2 in
     let e3 = extract_mlexpr g e3 in
     mk_assign (mk_expr_index e1 e2) e3
+  | S.MLE_App ({expr=S.MLE_TApp ({expr=S.MLE_Name p}, [_])}, [e1; e2])
+    when S.string_of_mlpath p = "Pulse.Lib.Rust.Vec.alloc" ->
+    let e1 = extract_mlexpr g e1 in
+    let e2 = extract_mlexpr g e2 in
+    mk_call (Expr_path vec_new_fn) [e1; e2]
+  | S.MLE_App ({expr=S.MLE_TApp ({expr=S.MLE_Name p}, [_])}, [e; _])
+    when S.string_of_mlpath p = "Pulse.Lib.Rust.Vec.free" ->
+    let e = extract_mlexpr g e in
+    mk_call (Expr_path "drop") [e]
   | S.MLE_App ({expr=S.MLE_Name p}, [{expr=S.MLE_Fun (_, cond)}; {expr=S.MLE_Fun (_, body)}])
     when S.string_of_mlpath p = "Pulse.Lib.Core.while_" ->
     let expr_while_cond = extract_mlexpr g cond in
